Fix string proof and move CopyByte T towards data_to_word
Progress on #499

compiler/backend/semantics/bviSemScript.sml
@@ -86,7 +86,7 @@ val do_app_aux_def = Define `
     | (String _, _) => NONE
     | (FromListByte, _) => NONE
     | (ConcatByteVec, _) => NONE
-    | (CopyByte T, _) => NONE
+    (* | (CopyByte T, _) => NONE *)
     | _ => SOME NONE`
 
 val do_install_def = Define `
