compiler/backend/bvl_to_bviScript.sml
@@ -209,7 +209,7 @@ local val compile_op_quotation = `
                            [Var 1; Op (Const 0) []] NONE;
                          Var 0; Var 1])
     | String str =>
-        Let [Op (RefByte T) [Op (Const 0) c1; Op (WordFromInt 8) [compile_int (&(LENGTH str))]]]
+        Let [Op (RefByte T) [Op (WordConst (fixwidth 8 [])) c1; compile_int (&(LENGTH str))]]
           (Let (MAPi (λn c. Op UpdateByte [Op (WordConst (fixwidth 8 (n2v (ORD c)))) []; compile_int (&n); Var 0]) str)
             (Var (LENGTH str)))
     | FromListByte =>
@@ -231,11 +231,11 @@ local val compile_op_quotation = `
                [Op (Const 0) [];
                 Call 0 (SOME SumListLength_location)
                   [Var 0; Op (Const 0) []] NONE]] NONE)
-    | CopyByte T => (* TODO: this should eventually be implemented in data_to_word instead for efficiency *)
+(*    | CopyByte T => (* TODO: this should eventually be implemented in data_to_word instead for efficiency *)
       Let (if LENGTH c1 < 3 then (c1 ++ REPLICATE 3 (Op (Const 0) [])) else c1)
         (Let [Op (RefByte T) [Op (Const 0) []; Var 0]]
            (Let [Op (CopyByte F) [Op (Const 0) []; Var 0; Var 1; Var 2; Var 3]]
-             (Var 1)))
+             (Var 1))) *)
     | Label l => Op (Label (bvl_num_stubs + bvl_to_bvi_namespaces * l)) c1
     | _ => Op op c1`
 in
